Gamma definitions inductive

Classes/Galois.v
@@ -4,14 +4,15 @@ Require Import Instances.Preorder.
 
 Implicit Type A B : Type.
 
-Class Galois A B `{PreorderedSet B} : Type :=
+Class Galois A B : Type :=
 {
+  galois_preorder :> PreorderedSet B;
   gamma : B -> A -> Prop;
   gamma_monotone : monotone gamma;
 
 }.
-Arguments Build_Galois A B {_ _ _}.
-Arguments gamma {_ _ _ _}.
+Arguments gamma : simpl never.
+Hint Extern 10 (gamma _ _) => constructor : soundness.
 
 Ltac gamma_destruct := repeat
   match goal with
@@ -21,12 +22,10 @@ Ltac gamma_destruct := repeat
 Lemma widen {A B} `{Galois B A}: forall (a a' : A) (b : B), 
     preorder a a' -> gamma a b -> gamma a' b.
 Proof.
-  intros.
-  pose proof gamma_monotone.
-  unfold monotone in H3. apply H3 in H1.
-  simpl in H1. 
-  unfold preordered_set_le in H1.
-  auto.
+  intros a a' b Hpre Hgamma.
+  pose proof gamma_monotone as Hmono.
+  unfold monotone in Hmono. apply Hmono in Hpre.
+  destruct Hpre. auto with soundness.
 Qed.
 
 Ltac apply_widen :=
