Classes/SoundMonad.v
@@ -6,20 +6,19 @@ Require Import Classes.Galois.
 Require Import Instances.Galois.
 
 Section monad_sound. 
-  Context (M M' : Type → Type) `{Monad M, Monad M'}.
-  Context {A A' B B' : Type} `{Galois A A', Galois B B'}.
-  Context `{Galois (M A) (M' A'), Galois (M B) (M' B')}.
-  Context `{Galois (M (A → B)) (M' (A' → B'))}.
+  Context M M' `{Monad M, Monad M'}.
+  Hypothesis M_galois : ∀ A A' : Type, Galois A A' → Galois (M A) (M' A').
 
-  Class SoundMonads : Type :=
-  {
-    fmap_sound : gamma (B:=(A' → B') → M' A' → M' B')
-                  fmap fmap;
-    pure_sound : gamma (B:=A' → M' A') pure pure;
-    app_sound  : gamma (B:=M' (A' → B') → M' A' → M' B')
-                  app app; 
-    bind_sound : gamma (B:=M' A' → (A' → M' B') → M' B')
-                  bindM bindM;
+  Class SoundMonad : Type := {
+    fmap_sound : ∀ {A A' B B' : Type} `{Galois A A', Galois B B'}, 
+      gamma (B:=(A' → B') → M' A' → M' B') fmap fmap;
+    pure_sound : ∀ {A A': Type} `{Galois A A'},
+      gamma (B:= (A' → M' A')) (A:=A → M A) pure pure;
+    app_sound : ∀ {A A' B B' : Type} `{Galois A A', Galois B B'}, 
+      gamma (B:=M' (A' → B') → M' A' → M' B') app app;
+    bind_sound : ∀ {A A' B B' : Type} `{Galois A A', Galois B B'},
+      gamma (B:=M' A' → (A' → M' B') → M' B') bindM bindM;
   }.
 End monad_sound.
+Arguments SoundMonad M M' [H H0 M_galois].
 Hint Resolve fmap_sound pure_sound app_sound bind_sound : soundness.
