Classes/Monad.v
@@ -23,6 +23,7 @@ Class Monad M : Type :=
     bindM (f <$> x) g = bindM x (f ∘ g);
   bind_pass : ∀ {A B} (ma : M A) (mb : M B), ma >> mb = bindM ma (λ _, mb);
 }.
+Hint Unfold bindM : soundness.
 
 Hint Rewrite @bind_id_left @bind_id_right @bind_assoc @bind_app : soundness.
 
